Add type checking to spec translator.
In order to deal with things like field selection and correct treatment of references, we need type information for the translated SpecExp's. This change adds type checking to the translator and extends the test suite.

The type checking also has the added benefit that we report context errors in the spec language directly at the source instead of via the generated boogie. Right now, the tool bails out on the first type error, but the code is setup so systematic collection of errors with source level backlink can be added in subsequent PRs.

Closes: #2083
Approved by: sblackshear

language/move-prover/bytecode-to-boogie/src/translator.rs
@@ -2,6 +2,16 @@
 // SPDX-License-Identifier: Apache-2.0
 
 //! This module translates the bytecode of a module to Boogie code.
+//!
+//! TODO: there is several cleanup to do in this module.
+//!
+//! 1. We should generalize the state and various helper functions into an 'environment'/'context'
+//!    abstraction which is shared between phases like bytecode and spec translation. This
+//!    environment should. among other things, allow to collect diagnostics related to the
+//!    translation.
+//! 2. We should factor out basic functions which represent interacting with the boogie model,
+//!    for example, how to construct a TypeValue from a SignatureToken, how to access memory,
+//!    and so on.
 
 use crate::spec_translator::SpecTranslator;
 use bytecode_source_map::source_map::ModuleSourceMap;
@@ -34,8 +44,6 @@ use vm::{
 /// Represents information about a module.
 #[derive(Debug)]
 pub struct ModuleInfo {
-    /// The index of this module in the module handle table.
-    pub index: usize,
     /// The name of this module.
     pub name: String,
     /// List of function specifications, in function declaration order.
@@ -45,14 +53,13 @@ pub struct ModuleInfo {
 /// Represents information about a function.
 #[derive(Debug)]
 pub struct FunctionInfo {
-    // Index of this function in the module vector.
-    pub index: usize,
-    // Name of this function.
-    pub name: String,
-    // List of type argument names.
-    pub type_arg_names: Vec<String>,
-    // List of argument names.
+    /// Index of this function in the function definition table.
+    pub index: FunctionDefinitionIndex,
+    /// List of function argument names. Those aren't present in the bytecode but we obtain them
+    /// from the AST.
     pub arg_names: Vec<String>,
+    /// List of type argument names.
+    pub type_arg_names: Vec<String>,
     /// List of specification conditions.
     pub specification: Vec<Condition>,
 }
@@ -69,6 +76,7 @@ pub struct BoogieTranslator<'a> {
 }
 
 pub struct ModuleTranslator<'a> {
+    pub parent: &'a BoogieTranslator<'a>,
     pub module: &'a VerifiedModule,
     pub module_info: &'a ModuleInfo,
     pub source_map: &'a ModuleSourceMap<Loc>,
@@ -263,7 +271,7 @@ impl<'a> BoogieTranslator<'a> {
 
 impl<'a> ModuleTranslator<'a> {
     pub fn new(
-        parent: &BoogieTranslator,
+        parent: &'a BoogieTranslator,
         module: &'a VerifiedModule,
         module_info: &'a ModuleInfo,
         source_map: &'a ModuleSourceMap<Loc>,
@@ -275,6 +283,7 @@ impl<'a> ModuleTranslator<'a> {
             all_type_strs.insert(struct_name);
         }
         Self {
+            parent,
             module,
             module_info,
             source_map,
@@ -798,7 +807,7 @@ impl<'a> ModuleTranslator<'a> {
         let function_info = &self.module_info.function_infos[idx];
         format!(
             "\n{}",
-            &SpecTranslator::new(self.module, function_info).translate()
+            &SpecTranslator::new(self.parent.modules, self.module, function_info).translate()
         )
     }
 
